src/Init/Data/Array/Zip.lean
@@ -118,7 +118,7 @@ theorem zipWith_foldl_eq_zip_foldl {f : α → β → γ} {i : δ} :
 theorem zipWith_eq_empty_iff {f : α → β → γ} {as : Array α} {bs : Array β} : zipWith f as bs = #[] ↔ as = #[] ∨ bs = #[] := by
   cases as <;> cases bs <;> simp
 
-@[grind =]
+@[simp, grind =]
 theorem map_zipWith {δ : Type _} {f : α → β} {g : γ → δ → α} {cs : Array γ} {ds : Array δ} :
     map f (zipWith g cs ds) = zipWith (fun x y => f (g x y)) cs ds := by
   cases cs
@@ -353,6 +353,15 @@ theorem map_zipWithAll {δ : Type _} {f : α → β} {g : Option γ → Option �
 
 @[deprecated zipWithAll_replicate (since := "2025-03-18")]
 abbrev zipWithAll_mkArray := @zipWithAll_replicate
+
+/-! ### zipWithM -/
+
+@[simp, grind =]
+theorem zipWithM_eq_mapM_id_zipWith {m : Type v → Type w} [Monad m] [LawfulMonad m] {f : α → β → m γ} {as : Array α} {bs : Array β} :
+    zipWithM f as bs = mapM id (zipWith f as bs) := by
+  cases as
+  cases bs
+  simp [List.zipWithM_toArray, ← List.zipWithM'_eq_zipWithM]
 
 /-! ### unzip -/
 
